bin_repeater.v
@@ -15,7 +15,7 @@ Open Scope N_scope.
 =============================================================================
  *)
 
-(* We introduce "repeater" and how to use it to redefine the hyperoperations
+(* We introduce "bin_repeater" and how to use it to redefine the bin_hyperoperations
    and Ackermann function.
    We also prove several results about the value of hypeopererations at small
    numbers and levels, which are treated as known in the paper but need to be
@@ -26,21 +26,21 @@ Open Scope N_scope.
 
 (* ****** REPEATER ********************************* *)
 
-Definition repeater (f : N -> N) (a : N) (n : N) : N :=
+Definition bin_repeater_from (f : N -> N) (a : N) (n : N) : N :=
   match n with
   | 0      => a
-  | Npos p => let fix repeater_pos (g : N -> N) (p : positive) (a' : N) : N :=
+  | Npos p => let fix bin_repeater_pos (g : N -> N) (p : positive) (a' : N) : N :=
                match p with
                | xH    => g a'
-               | xO p' => let g' := repeater_pos g p' in g' (g' a')
-               | xI p' => let g' := repeater_pos g p' in g (g' (g' a'))
-               end in repeater_pos f p a
+               | xO p' => let g' := bin_repeater_pos g p' in g' (g' a')
+               | xI p' => let g' := bin_repeater_pos g p' in g (g' (g' a'))
+               end in bin_repeater_pos f p a
   end.
 
 (* Repeater is a functional way to look at repeat
    See "repeat" in "prelims.v" *)
-Theorem repeater_repeat :
-    forall a f n, repeater f a n = repeat f (N.to_nat n) a.
+Theorem bin_repeater_repeat :
+    forall a f n, bin_repeater_from f a n = repeat f (N.to_nat n) a.
 Proof.
   intros a f n. destruct n; trivial. simpl.
   generalize dependent a.
@@ -52,24 +52,24 @@ Qed.
 
 (*
 (* Repeater on N is consistent with its counterpart on nat *)
-Theorem repeater_Nnat : 
-    forall a f, repeater f a =
-    to_N_func (repeater.repeater_from (to_nat_func f) (N.to_nat a)).
+Theorem bin_repeater_Nnat : 
+    forall a f, bin_repeater_from f a =
+    to_N_func (repeater.bin_repeater_from (to_nat_func f) (N.to_nat a)).
 Proof.
   intros a f. apply functional_extensionality; intro n.
-  unfold to_N_func. rewrite repeater_repeat.
-  rewrite repeater.repeater_from_repeat.
+  unfold to_N_func. rewrite bin_repeater_repeat.
+  rewrite repeater.bin_repeater_from_repeat.
   remember (N.to_nat n) as m. clear Heqm. unfold to_nat_func.
   induction m; simpl; [ |rewrite <- IHm]; rewrite N2Nat.id; trivial.
 Qed.
 *)
 
 (* Repeater on N is consistent with its counterpart on nat *)
-Theorem repeater_Nnat : 
-    forall a f n, repeater f a n =
+Theorem bin_repeater_Nnat : 
+    forall a f n, bin_repeater_from f a n =
     N.of_nat (repeater.repeater_from (to_nat_func f) (N.to_nat a) (N.to_nat n)).
 Proof.
-  intros a f n. rewrite repeater_repeat.
+  intros a f n. rewrite bin_repeater_repeat.
   rewrite repeater.repeater_from_repeat.
   remember (N.to_nat n) as m. clear Heqm. unfold to_nat_func.
   induction m; simpl; [ |rewrite <- IHm]; rewrite N2Nat.id; trivial.
@@ -78,57 +78,57 @@ Qed.
 
 (* ****** HYPEROPS ********************************* *)
 
-(* A function to summarize the initial values of the hyperoperations *)
-Definition hyperop_init (a : N) (n : nat) : N :=
+(* A function to summarize the initial values of the bin_hyperoperations *)
+Definition bin_hyperop_init (a : N) (n : nat) : N :=
   match n with 0%nat => a | 1%nat => 0 | _ => 1 end.
 
-(* Our definition for hyperops using repeater *)
-Fixpoint hyperop (a : N) (n : nat) (b : N) : N :=
+(* Our definition for bin_hyperops using bin_repeater_from *)
+Fixpoint bin_hyperop (a : N) (n : nat) (b : N) : N :=
   match n with
   | 0%nat => 1 + b
-  | S n'  => repeater (hyperop a n') (hyperop_init a n') b
+  | S n'  => bin_repeater_from (bin_hyperop a n') (bin_hyperop_init a n') b
   end.
 
-(* A handy theorem to transform goals involving hyperops *)
-Lemma hyperop_recursion :
+(* A handy theorem to transform goals involving bin_hyperops *)
+Lemma bin_hyperop_recursion :
   forall (n : nat) (a : N),
-    hyperop a (S n) = repeater (hyperop a n) (hyperop_init a n).
+    bin_hyperop a (S n) = bin_repeater_from (bin_hyperop a n) (bin_hyperop_init a n).
 Proof. intros. apply functional_extensionality. intro b. trivial. Qed.
 
-(* Proof that the two hyperops are the same *)
-Theorem hyperop_correct :
-  forall n a b, hyperop a n b = N.of_nat (repeater.hyperop (N.to_nat a) n (N.to_nat b)).
+(* Proof that the two bin_hyperops are the same *)
+Theorem bin_hyperop_correct :
+  forall n a b, bin_hyperop a n b = N.of_nat (repeater.hyperop (N.to_nat a) n (N.to_nat b)).
 Proof.
   intros n a. induction n; intro b.
-  - unfold hyperop. unfold repeater.hyperop. lia.
-  - rewrite hyperop_recursion.
+  - unfold bin_hyperop. unfold repeater.hyperop. lia.
+  - rewrite bin_hyperop_recursion.
     replace (repeater.hyperop (N.to_nat a) (S n) (N.to_nat b)) with
     (repeater.repeater_from (repeater.hyperop (N.to_nat a) n)
                           (repeater.hyperop_init (N.to_nat a) n)
                           (N.to_nat b)) by trivial.
     replace (repeater.hyperop_init (N.to_nat a) n) with
-    (N.to_nat (hyperop_init a n)) by repeat (destruct n; trivial).
-    rewrite repeater_Nnat. repeat f_equal.
+    (N.to_nat (bin_hyperop_init a n)) by repeat (destruct n; trivial).
+    rewrite bin_repeater_Nnat. repeat f_equal.
     apply functional_extensionality; intro c.
     unfold to_nat_func. rewrite IHn. repeat rewrite Nat2N.id. trivial.
 Qed.
 
-(* The first few functions in the hyperops. Useful for pointing out
+(* The first few functions in the bin_hyperops. Useful for pointing out
    their inverse specifically *)
 
-Lemma hyperop_1 : forall a b, hyperop a 1 b = b + a.
+Lemma bin_hyperop_1 : forall a b, bin_hyperop a 1 b = b + a.
 Proof.
-  intros. rewrite hyperop_correct. rewrite repeater.hyperop_1. lia.
+  intros. rewrite bin_hyperop_correct. rewrite repeater.hyperop_1. lia.
 Qed.
 
-Lemma hyperop_2 : forall a b, hyperop a 2 b = b * a.
+Lemma bin_hyperop_2 : forall a b, bin_hyperop a 2 b = b * a.
 Proof.
-  intros. rewrite hyperop_correct. rewrite repeater.hyperop_2. lia.
+  intros. rewrite bin_hyperop_correct. rewrite repeater.hyperop_2. lia.
 Qed.
 
-Lemma hyperop_3 : forall a b, hyperop a 3 b = a ^ b.
+Lemma bin_hyperop_3 : forall a b, bin_hyperop a 3 b = a ^ b.
 Proof.
-  intros. rewrite hyperop_correct. rewrite repeater.hyperop_3.
+  intros. rewrite bin_hyperop_correct. rewrite repeater.hyperop_3.
   remember (N.to_nat a) as a0. replace a with (N.of_nat a0) by lia. clear Heqa0.
   remember (N.to_nat b) as b0. replace b with (N.of_nat b0) by lia. clear Heqb0.
   induction b0; trivial. replace (N.of_nat (S b0)) with (1 + N.of_nat b0) by lia.
@@ -136,9 +136,9 @@ Proof.
 Qed.
 
 (* A beautiful result about hypeops value at b = 1.
-   Used in the proof of the theorem "ack_hyperop",
+   Used in the proof of the theorem "ack_bin_hyperop",
    which is also just for aesthetics *)
-Lemma hyperop_n_1 : forall n a, (2 <= n)%nat -> hyperop a n 1 = a.
+Lemma bin_hyperop_n_1 : forall n a, (2 <= n)%nat -> bin_hyperop a n 1 = a.
 Proof.
   intros n a Hn. do 2 (destruct n; [omega|]).
   clear Hn. induction n; trivial.
@@ -146,12 +146,12 @@ Qed.
 
 (* ****** ACKERMANN FUNCTION ********************************* *)
 
-(* Our definition using repeater *)
+(* Our definition using bin_repeater_from *)
 Definition ackermann (n m : N) : N :=
   let fix ack_nat (n0 : nat) (m0 : N) : N :=
    match n0 with
    | 0%nat => 1 + m0
-   | S n1  => repeater (ack_nat n1) (ack_nat n1 1) m0
+   | S n1  => bin_repeater_from (ack_nat n1) (ack_nat n1 1) m0
    end in ack_nat (N.to_nat n) m.
 
 (* Proof that the above are the same *)
@@ -160,7 +160,7 @@ Theorem ackermann_correct : forall n m,
 Proof.
   intros n m. unfold ackermann. unfold repeater.ackermann.
   generalize dependent m. induction (N.to_nat n); intro m; [lia| ].
-  rewrite repeater_Nnat. repeat f_equal;
+  rewrite bin_repeater_Nnat. repeat f_equal;
   [unfold to_nat_func; apply functional_extensionality; intro p| ];
   rewrite IHn0; repeat rewrite Nat2N.id; trivial.
 Qed.
